refactor

src/tm.lean
@@ -1,6 +1,5 @@
-import tactic data.vector.zip algebra.big_operators.basic algebra.big_operators.norm_num
+import tactic data.vector.basic data.vector.zip algebra.big_operators.basic algebra.big_operators.norm_num
 import vorspiel
-
 
 open_locale big_operators
 
@@ -16,6 +15,8 @@ inductive language (Γ : Type u)
 notation `␣` := language.blank 
 notation `␤` := language.start
 
+instance {Γ : Type u} : inhabited (language Γ) := ⟨␣⟩
+
 class state_lang (Q : Type u) :=
 (start : Q)
 (halt : Q)
@@ -24,27 +25,12 @@ instance {Q R} [state_lang Q] [state_lang R] : state_lang (Q ⊕ R) := ⟨sum.in
 
 end turing_machine
 
-def option.to_language {Γ : Type u} : option Γ → turing_machine.language Γ
-| none     := ␣
-| (some x) := turing_machine.language.chr x
-
 namespace turing_machine
 open state_lang
 
-namespace TM
-
-inductive deg 
-| stay  : deg
-| right : deg
-| left  : deg
-
-end TM
-
-class tape_class (α : Type u) := (input : α) (output : α)
-
 variables
   (Γ : Type u) -- 言語
-  (Q : Type v) -- 状態
+  (Q : Type v) [state_lang Q] -- 状態
   (ι : ℕ) -- テープの数
 
 inductive instruction
@@ -52,354 +38,161 @@ inductive instruction
 | right : instruction
 | left  : instruction
 
+instance : inhabited instruction := ⟨instruction.stay⟩
+
 @[simp] def instruction.apply : instruction → ℕ → ℕ
 | instruction.stay  ι := ι
 | instruction.right ι := ι + 1
 | instruction.left  ι := ι - 1
 
+@[simp] lemma instruction.apply_default (n) : instruction.apply default n = n := rfl
+
+@[simp] lemma instruction.default_nth (ι : ℕ) (i) : (default : vector instruction ι).nth i = instruction.stay :=
+by { unfold default, simp }
+
 structure word :=
-(cond : Q × vector Γ ι)
-(cons : Q × vector (Γ × instruction) ι)
+(c : Q)
+(z : vector Γ ι)
+(u : vector instruction ι)
+(q : Q)
+(x : vector Γ ι)
 
-infix ` ▷ `:80 := word.mk
-
-structure line :=
-(tape : ℕ → Γ)
-(head : ℕ)
-
-@[ext] lemma line.ext (l₁ l₂ : line Γ) (et : l₁.tape = l₂.tape) (eh : l₁.head = l₂.head) : l₁ = l₂ :=
-by { rcases l₁; rcases l₂, simp at et eh, simp[eh, et] }
+notation `⟮` c `, ` z `; ` u ` | ` q `, ` x `⟯`:80 := word.mk c z u q x
 
 structure model :=
 (state : Q) 
-(lines : vector (line Γ) ι)
+(tape : vector (ℕ → Γ) ι)
+(head : vector ℕ ι)
 
+notation `⟦` q `, ` T `, ` H `⟧` := model.mk q T H
 
-abbreviation sentence := set (word Γ Q ι)
+structure sentence :=
+(carrier : set (word Γ Q ι))
+(proper' : ∀ c z u q x, ⟮c, z; u | q, x⟯ ∈ carrier → q ≠ state_lang.halt ∧ c ≠ state_lang.start)
+
+namespace sentence
+variables {Γ Q ι}
+variables (σ : sentence Γ Q ι)
+
+instance : set_like (sentence Γ Q ι) (word Γ Q ι) := ⟨sentence.carrier,by { rintros ⟨_, _⟩ ⟨_, _⟩, simp }⟩
+
+lemma mem_def (w : word Γ Q ι) : w ∈ σ ↔ w ∈ σ.carrier := iff.rfl
+
+lemma proper {c z u q x} : ⟮c, z; u | q, x⟯ ∈ σ → q ≠ state_lang.halt ∧ c ≠ state_lang.start := σ.proper' _ _ _ _ _
+
+@[simp] lemma start_notin (c z u x) : ⟮c, z; u | halt, x⟯ ∉ σ := λ A, by simpa using σ.proper A
+
+@[simp] lemma halt_notin (z u q x) : ⟮start, z; u | q, x⟯ ∉ σ := λ A, by simpa using σ.proper A 
+
+end sentence
 
 variables {Γ Q ι}
 
 namespace model
 variables (σ : sentence Γ Q ι)
 
+
 @[ext] lemma ext : ∀ {m₁ m₂ : model Γ Q ι}
-  (input : m₁.lines = m₂.lines)
-  (state : m₁.state = m₂.state), m₁ = m₂
-| ⟨q₁, L₁⟩ ⟨q₂, L₂⟩ tape state :=
-  by { simp, split, { exact state }, { funext, exact tape }  }
+  (hs : m₁.state = m₂.state)
+  (ht : m₁.tape = m₂.tape)
+  (hh : m₁.head = m₂.head), m₁ = m₂
+| ⟦q₁, T₁, H₁⟧ ⟦q₂, T₂, H₂⟧ hs ht hh :=
+  by { simp at hs ht hh, simp[hs, ht, hh] }
 
-def read (m : model Γ Q ι) : vector Γ ι := m.lines.map (λ l, l.1 l.2)
+def read (T : vector (ℕ → Γ) ι) (H : vector ℕ ι) : vector Γ ι := @vector.zip_with (ℕ → Γ) ℕ Γ ι (λ t h, t h) T H
 
-def snapshot (m : model Γ Q ι) : Q × vector Γ ι := ⟨m.state, m.lines.map (λ ⟨T, n⟩, T n)⟩
+@[simp] lemma read_nth (T : vector (ℕ → Γ) ι) (H : vector ℕ ι) (i) : (read T H).nth i = (T.nth i) (H.nth i) :=
+by simp[read]
 
-def reduct (q : Q) (z : vector (Γ × instruction) ι) : model Γ Q ι → model Γ Q ι
-| ⟨_, L⟩ :=
-  { lines := @vector.zip_with (line Γ) (Γ × instruction) (line Γ) ι
-      (λ ⟨T, h⟩ ⟨x, i⟩, ⟨λ n, if n = h then x else T n, i.apply h⟩) L z,
-    state := q }
+@[irreducible] def reduct_tape (T H) (x : vector Γ ι) : vector (ℕ → Γ) ι :=
+  @vector.zip_with3 (ℕ → Γ) ℕ Γ (ℕ → Γ) ι (λ t h x, λ n, if n = h then x else t n) T H x
 
-@[simp] lemma reduct_head (m : model Γ Q ι) (q : Q) (z : vector (Γ × instruction) ι) :
-  (reduct q z m).state = q := by cases m; simp[reduct]
+@[irreducible] def reduct_head (H) (u : vector instruction ι) : vector ℕ ι :=
+  vector.zip_with instruction.apply u H
 
-lemma reduct_lines_nth (m : model Γ Q ι) (q : Q) (z : vector (Γ × instruction) ι) (i : fin ι) :
-  (reduct q z m).lines.nth i = ⟨λ n, if n = (m.lines.nth i).2 then (z.nth i).1 else (m.lines.nth i).1 n, (z.nth i).2.apply (m.lines.nth i).2⟩ :=
-by { rcases m with ⟨_, L⟩, rcases eL : L.nth i with ⟨T, h⟩, rcases ez: z.nth i with ⟨x, ins⟩, simp[eL, ez, reduct] }
+@[simp] lemma reduct_tape_nth (T H) (x : vector Γ ι) (i) :
+  (reduct_tape T H x).nth i = (λ n, if n = H.nth i then x.nth i else T.nth i n) :=
+by simp[reduct_tape]
 
+@[simp] lemma reduct_head_nth  (H) (u : vector instruction ι) (i) :
+  (reduct_head H u).nth i = (u.nth i).apply (H.nth i) :=
+by simp[reduct_head]
 
 inductive reduction : model Γ Q ι → model Γ Q ι → Prop
-| intro : ∀ (m : model Γ Q ι) (q : Q) (z : vector (Γ × instruction) ι),
-    ⟨m.state, m.read⟩ ▷ ⟨q, z⟩ ∈ σ → reduction m (reduct q z m)
-  
+| intro : ∀ (q : Q) (T : vector (ℕ → Γ) ι) (H : vector ℕ ι) (c : Q) (z : vector Γ ι) (u : vector instruction ι),
+    ⟮c, z; u | q, read T H⟯ ∈ σ → reduction ⟦q, T, H⟧ ⟦c, reduct_tape T H z, reduct_head H u⟧
+
 notation m₀ ` ⟶¹[`:60  σ `] ` :0 m₁ := reduction σ m₀ m₁ 
 
 def is_halt (m : model Γ Q ι) : Prop := ∀ m', ¬m ⟶¹[σ] m'
 
-inductive time_reductions : ℕ → model Γ Q ι → model Γ Q ι → Prop
-| zero : ∀ m, time_reductions 0 m m
-| succ : ∀ {ι m₀ m₁ m₂}, time_reductions ι m₀ m₁ → (m₁ ⟶¹[σ] m₂) → time_reductions ι.succ m₀ m₂
+def time_reductions : ℕ → model Γ Q ι → model Γ Q ι → Prop := relation.power (reduction σ) 
 
-attribute [simp] time_reductions.zero
+notation m₀ ` ⟶^(`:80 s `)[`  σ `] ` :80 m₁ := time_reductions σ s m₀ m₁ 
 
-notation m₀ ` ⟶^(`:80 s `)[`:80  σ `] ` :0 m₁ := time_reductions σ s m₀ m₁ 
+def time_bounded_reductions : ℕ → model Γ Q ι → model Γ Q ι → Prop := relation.power_le (reduction σ)
 
-def time_bounded_reductions (s : ℕ) (m m' : model Γ Q ι) : Prop := ∃ s' ≤ s, m ⟶^(s')[σ] m'
-notation m₀ ` ⟶^(≤ ` s `)[`:80  σ `] ` :0 m₁ := time_bounded_reductions σ s m₀ m₁ 
+notation m₀ ` ⟶^(≤ `:80 s `)[`  σ `] ` :80 m₁ := time_bounded_reductions σ s m₀ m₁ 
 
-def time_bounded_reductions_halt (s : ℕ) (m m' : model Γ Q ι) : Prop := is_halt σ m' ∧ ∃ s' ≤ s, m ⟶^(s')[σ] m'
-notation m₀ ` ⟶^(≤ ` s `)[`:80  σ `]↓ ` :0 m₁ := time_bounded_reductions_halt σ s m₀ m₁ 
+def time_bounded_reductions_halt (s : ℕ) (m m' : model Γ Q ι) : Prop := is_halt σ m' ∧ m ⟶^(≤ s)[σ] m'
 
-def reductions (m m' : model Γ Q ι) : Prop := ∃ s : ℕ, m ⟶^(s)[σ] m' 
+notation m₀ ` ⟶^(≤ `:80 s `)[`  σ `]↓ ` :80 m₁ := time_bounded_reductions_halt σ s m₀ m₁ 
+
+def is_halt_in_step (s : ℕ) (m : model Γ Q ι) : Prop := ∀ (m') (s' > s), ¬ m ⟶^(s')[σ] m' 
+
+def reductions : model Γ Q ι → model Γ Q ι → Prop := relation.trans_gen (reduction σ) 
 
 notation m₀ ` ⟶*[`:80  σ `] ` :0 m₁ := reductions σ m₀ m₁ 
-
-def converge (m₀ m₁ : model Γ Q ι) : Prop := is_halt σ m₁ ∧ (m₀ ⟶*[σ] m₁)
-
-notation m₀ ` ⟶ᵗ[`:80 σ `] ` :0 m₁ := converge m₀ m₁
 
 end model
 
 variables {Γ Q ι} 
-def sentence.deterministic (σ : sentence Γ Q ι) : Prop := ∀ q q₁ q₂, q ▷ q₁ ∈ σ → q ▷ q₂ ∈ σ → q₁ = q₂
-
-def sentence.proper [state_lang Q] (σ : sentence Γ Q ι) : Prop :=
-  ∀ w₁ w₂, w₁ ▷ w₂ ∈ σ → w₁.1 ≠ state_lang.halt ∧ w₂.1 ≠ state_lang.start
+def sentence.deterministic (σ : sentence Γ Q ι) : Prop :=
+∀ ⦃q x c₁ c₂ z₁ z₂ u₁ u₂⦄, ⟮c₁, z₁; u₁ | q, x⟯ ∈ σ → ⟮c₂, z₂; u₂ | q, x⟯ ∈ σ → c₁ = c₂ ∧ z₁ = z₂ ∧ u₁ = u₂
 
 namespace sentence
+
+inductive of_fun_aux (δ : Q × vector Γ ι → option (Q × vector Γ ι × vector instruction ι)) : set (word Γ Q ι)
+| intro : ∀ {q x c z u}, δ ⟨q, x⟩ = some ⟨c, z, u⟩ → of_fun_aux ⟮c, z; u | q, x⟯
+
+def of_fun (δ : Q × vector Γ ι → option (Q × vector Γ ι × vector instruction ι))
+  (H : ∀ {q x c z u}, δ ⟨q, x⟩ = some ⟨c, z, u⟩ → q ≠ halt ∧ c ≠ start) : sentence Γ Q ι :=
+{ carrier := of_fun_aux δ,
+  proper' := λ c z u q x, by { rintro ⟨_, _, _, _, _, h⟩, exact H h } }
+
+namespace of_fun
+variables (δ : Q × vector Γ ι → option (Q × vector Γ ι × vector instruction ι))
+
+lemma carrier_eq {H} : (of_fun δ H).carrier = of_fun_aux δ := rfl
+
+@[simp] lemma mem_iff {H} {c z u q x} : ⟮c, z; u | q, x⟯ ∈ of_fun δ H ↔ δ ⟨q, x⟩ = some ⟨c, z, u⟩ :=
+by { simp[sentence.mem_def], split,
+  { rintros ⟨_, _, _, _, _, h⟩, exact h }, { intros h, exact of_fun_aux.intro h } }
+
+lemma of_fn.deterministic {H} : deterministic (of_fun δ H) :=
+λ _ _ _ _ _ _ _ _, by { simp, intros h₁ h₂, simpa[h₁] using h₂ }
+
+end of_fun
 
 namespace deterministic
 variables {σ : sentence Γ Q ι} {m₁ m₂ : model Γ Q ι}
 
-lemma reduction (d : deterministic σ) {m m₁ m₂}
-  (h₁ : m ⟶¹[σ] m₁) (h₂ : m ⟶¹[σ] m₂) : m₁ = m₂ :=
+lemma reduction (d : deterministic σ) : relation.deterministic (model.reduction σ) := λ m m₁ m₂ h₁ h₂,
 begin
-  rcases h₁ with ⟨_, q₁, z₁, w₁⟩,
-  rcases h₂ with ⟨_, q₂, z₂, w₂⟩,
-  have : q₁ = q₂ ∧ z₁ = z₂, by simpa using d _ _ _ w₁ w₂,
-  rcases this with ⟨rfl, rfl, rfl⟩,
+  rcases h₁ with ⟨q₁, T₁, H₁, c₁, z₁, u₁, mem₁⟩,
+  rcases h₂ with ⟨q₂, T₂, H₂, c₂, z₂, u₂, mem₂⟩,
+  rcases d mem₁ mem₂ with ⟨rfl, rfl, rfl⟩,
   refl
 end
 
-lemma time_reductions (d : deterministic σ) {m m₁ m₂} {s} (h₁ : m ⟶^(s)[σ] m₁) (h₂ : m ⟶^(s)[σ] m₂) :
-  m₁ = m₂ :=
-begin
-  induction s with s IH generalizing m₁ m₂,
-  { rcases h₁, rcases h₂, refl },
-  { rcases h₁ with (_ | ⟨_, _, m₁₁, _, h_₁₁, h₁₁_₁⟩),
-    rcases h₂ with (_ | ⟨_, _, m₂₁, _, h_₂₁, h₂₁_₂⟩),
-    have : m₁₁ = m₂₁, from IH h_₁₁ h_₂₁, rcases this with rfl,
-    exact reduction @d h₁₁_₁ h₂₁_₂ }
-end
+lemma time_reductions (d : deterministic σ) {n} : relation.deterministic (model.time_reductions σ n) :=
+relation.power.deterministic (reduction @d)
 
 end deterministic
 
 end sentence
 
-namespace model
-open sentence sentence.deterministic
-variables {m₁ m₂ m₃ : model Γ Q ι} {σ : sentence Γ Q ι}
-
-@[simp] lemma time_bounded_reductions.refl {s} : m₁ ⟶^(≤ s)[σ] m₁ :=
-⟨0, zero_le s, time_reductions.zero m₁⟩
-
-lemma time_bounded_reductions.of_le {s₁ s₂} (h : m₁ ⟶^(≤ s₁)[σ] m₂) (le : s₁ ≤ s₂) :
-  m₁ ⟶^(≤ s₂)[σ] m₂ := 
-by rcases h with ⟨s, le_s, h⟩; refine ⟨s, le_trans le_s le, h⟩
-
-lemma time_reductions.add {s₁ s₂} (h₁ : m₁ ⟶^(s₁)[σ] m₂) (h₂ : m₂ ⟶^(s₂)[σ] m₃) :
-  m₁ ⟶^(s₁ + s₂)[σ] m₃ :=
-begin
-  induction s₂ with s₂ IH generalizing s₁ m₁ m₂ m₃,
-  { rcases h₂, exact h₁ },
-  { rcases h₂ with (_| ⟨_, _, m₂₁, _, h₂_₂₁, h₂₁_₃⟩),
-  simpa using (IH h₁ h₂_₂₁).succ h₂₁_₃ }
-end
-
-lemma time_bounded_reductions.add {s₁ s₂} (h₁ : m₁ ⟶^(≤ s₁)[σ] m₂) (h₂ : m₂ ⟶^(≤ s₂)[σ] m₃) :
-  m₁ ⟶^(≤ s₁ + s₂)[σ] m₃ :=
-begin
-  rcases h₁ with ⟨t₁, le₁, h₁⟩,
-  rcases h₂ with ⟨t₂, le₂, h₂⟩,
-  refine ⟨t₁ + t₂, add_le_add le₁ le₂, h₁.add h₂⟩,
-end
-
-lemma time_bounded_reductions.sum {m : ℕ → model Γ Q ι} {s : ℕ → ℕ}
-  (h : ∀ k, m k ⟶^(≤ s k)[σ] m (k + 1)) (k : ℕ) : (m 0) ⟶^(≤ ∑ i in finset.range k, s i)[σ] (m k) :=
-by { induction k with k IH, { simp }, { simpa[finset.sum_range_succ] using IH.add (h k) } }
-
-lemma reduction.of_ss (r : m₁ ⟶¹[σ] m₂) {τ : sentence Γ Q ι} (ss : σ ⊆ τ) : m₁ ⟶¹[τ] m₂ :=
-by { rcases r with ⟨_, q, z, mem⟩, refine ⟨_, _, _, _⟩, exact ss mem }
-
-lemma time_reductions.of_ss {n} (r : m₁ ⟶^(n)[σ] m₂) {τ : sentence Γ Q ι} (ss : σ ⊆ τ) : m₁ ⟶^(n)[τ] m₂ :=
-by { induction n with n IH generalizing m₂, { rcases r, simp },
-     { rcases r with (_ | ⟨_, _, m₁₁, _, r₁_₁₁, r₁₁_₂⟩), exact (IH r₁_₁₁).succ (r₁₁_₂.of_ss ss) } }
-
-lemma time_bounded_reductions.of_ss {k} (r : m₁ ⟶^(≤ k)[σ] m₂) {τ : sentence Γ Q ι} (ss : σ ⊆ τ) : m₁ ⟶^(≤ k)[τ] m₂ :=
-by { rcases r with ⟨n, le, r⟩, refine ⟨n, le, r.of_ss ss⟩ }
-
-section
-variables {R : Type v} (f : Q → R)
-
-@[simp] def map_q : model Γ Q ι → model Γ R ι
-| ⟨q, L⟩ := ⟨f q, L⟩
-
-instance [has_coe Q R] : has_coe (model Γ Q ι) (model Γ R ι) := ⟨λ m, m.map_q coe⟩ 
-
-@[simp] def word.map_q : word Γ Q ι → word Γ R ι
-| (⟨q, w⟩ ▷ ⟨q', w'⟩) :=  ⟨f q, w⟩ ▷ ⟨f q', w'⟩
-
-variables (m m' : model Γ Q ι) {f}
-
-@[simp] lemma map_q_lines (m : model Γ Q ι) : (m.map_q f).lines = m.lines := by cases m; simp
-
-@[simp] lemma map_q_state (m : model Γ Q ι) : (m.map_q f).state = f m.state := by cases m; simp
-
-@[simp] lemma map_q_reduct (q : Q) (z : vector (Γ × instruction) ι) :
-  (reduct q z m).map_q f = reduct (f q) z (m.map_q f) := by cases m; simp[reduct]
-
-@[simp] lemma map_q_snapshot : (m.map_q f).read = m.read :=  by cases m; simp[read]
-
-variables (f)
-
-lemma reduction.map_q (h : m₁ ⟶¹[σ] m₂) (f : Q → R) : m₁.map_q f ⟶¹[word.map_q f '' σ] m₂.map_q f :=
-by { rcases h with ⟨_, q, w, mem⟩, simp, refine ⟨_, _, _, _⟩, simp, refine ⟨_, mem, by simp⟩ }
-
-lemma time_reductions.map_q {n} (h : m₁ ⟶^(n)[σ] m₂) (f : Q → R) : m₁.map_q f ⟶^(n)[word.map_q f '' σ] m₂.map_q f :=
-by { induction n with n IH generalizing m₂, { rcases h, simp },
-     { rcases h with (_ | ⟨_, _, m₁₁, _, r₁_₁₁, r₁₁_₂⟩), refine (IH r₁_₁₁).succ (r₁₁_₂.map_q f) } }
-
-lemma time_bounded_reduction.map_q {k} (h : m₁ ⟶^(≤ k)[σ] m₂) (f : Q → R) : m₁.map_q f ⟶^(≤ k)[word.map_q f '' σ] m₂.map_q f :=
-by { rcases h with ⟨n, le, r⟩, refine ⟨n, le, r.map_q f⟩ }
-
-variables {f}
-
-lemma deterministic.map_q (inj : function.injective f) (d : deterministic σ) : deterministic (word.map_q f '' σ) :=
-begin
-  rintros ⟨r, w⟩ ⟨r₁, w₁⟩ ⟨r₂, w₂⟩ h₁ h₂,
-  rcases h₁ with ⟨⟨⟨q, w'⟩, ⟨q₁, w₁'⟩⟩, mem₁, eq₁⟩,
-  have : f q = r ∧ w = w' ∧ f q₁ = r₁ ∧ w₁ = w₁', { simp at eq₁, simp[eq₁] },
-  rcases this with ⟨rfl, rfl, rfl, rfl⟩,
-  rcases h₂ with ⟨⟨⟨q', w'⟩, ⟨q₂, w₂'⟩⟩, mem₂, eq₂⟩,
-  have : f q' = f q ∧ w = w' ∧ f q₂ = r₂ ∧ w₂ = w₂', { simp at eq₂, simp[eq₂] },
-  rcases this with ⟨eq, rfl, rfl, rfl⟩,
-  have : q = q', from (inj eq).symm, rcases this with rfl,
-  have : q₁ = q₂ ∧ w₁ = w₂, by simpa using d _ _ _ mem₁ mem₂,
-  simp[this] 
-end
-
-end
-
-variables {R : Type v}
-
-inductive sentence.fix_q (q₁ q₂ : Q) : sentence Γ Q ι
-| intro : ∀ v : vector Γ ι, sentence.fix_q ((q₁, v) ▷ (q₂, v.map (λ x, (x, instruction.stay))))
-
-@[simp] lemma sentence.fix_q_mem (q₁ q₂ : Q) (v : vector Γ ι) :
-   ((q₁, v) ▷ (q₂, v.map (λ x, (x, instruction.stay)))) ∈ (sentence.fix_q q₁ q₂ : sentence Γ Q ι) :=
-sentence.fix_q.intro v
-
-lemma sentence.fix_q.deterministic (q₁ q₂ : Q) : deterministic (sentence.fix_q q₁ q₂ : sentence Γ Q ι) :=
-by { rintros w w₁ w₂ h₁ h₂, rcases h₁, rcases h₂, simp }
-
-lemma sentence.fix_q_reduction (q₁ q₂ : Q) (L : vector (line Γ) ι) : ⟨q₁, L⟩ ⟶¹[sentence.fix_q q₁ q₂] ⟨q₂, L⟩ :=
-begin
-  let v := (⟨q₁, L⟩ : model Γ Q ι).read,
-  let z := vector.map (λ (x : Γ), (x, instruction.stay)) v,
-  suffices : ⟨q₁, L⟩ ⟶¹[fix_q q₁ q₂] reduct q₂ z ⟨q₁, L⟩,
-  { have e: (⟨q₂, L⟩ : model Γ Q ι) = reduct q₂ z ⟨q₁, L⟩,
-    { ext; simp[reduct_lines_nth, v, read], by_cases e : x = (L.nth m).head; simp[e] },
-    simpa[e] using this },
-  have : (q₁, v) ▷ (q₂, z) ∈ fix_q q₁ q₂, from sentence.fix_q_mem q₁ q₂ v,
-  refine reduction.intro ⟨q₁, L⟩ q₂ z this
-end
-
-def deterministic.union {σ τ : sentence Γ Q ι} (dσ : deterministic σ) (dτ : deterministic τ)
-  (h : ∀ (w₁ w₂ : word Γ Q ι), w₁ ∈ σ → w₂ ∈ τ → w₁.cond = w₂.cond → w₁.cons = w₂.cons) : deterministic (σ ∪ τ) :=
-begin
-    rintros w w₁ w₂ h₁ h₂,
-   rcases h₁,
-   { rcases h₂, { exact dσ _ _ _ h₁ h₂ }, { simpa using h _ _ h₁ h₂ (by simp) } },
-   { rcases h₂, { simpa using (h _ _ h₂ h₁ (by simp)).symm }, { exact dτ _ _ _ h₁ h₂ } }
-end
-
-variables [state_lang Q] [state_lang R]
-
-def sentence.dsum (σ : sentence Γ Q ι) (τ : sentence Γ R ι) : sentence Γ (Q ⊕ R) ι :=
-(word.map_q sum.inl '' σ) ∪ (word.map_q sum.inr '' τ) ∪ (sentence.fix_q (sum.inl (halt : Q)) (sum.inr (start : R)))
-
-infix ` ⨁ `:80 := sentence.dsum
-
-lemma sentence.dsum.deterministic {σ : sentence Γ Q ι} {τ : sentence Γ R ι}
-  (proper : proper σ) (d₁ : deterministic σ) (d₂ : deterministic τ) : deterministic (σ ⨁ τ) :=
-begin
-  have : deterministic ((word.map_q sum.inl '' σ) ∪ (word.map_q sum.inr '' τ) : sentence Γ (Q ⊕ R) ι),
-  { refine deterministic.union (deterministic.map_q (sum.inl_injective) d₁) (deterministic.map_q (sum.inr_injective) d₂) _,
-    simp, rintros ⟨v₁, w₁⟩ ⟨v₂, w₂⟩ ⟨⟨q₁, u₁⟩, q'₁, u'₁⟩ mem₁,
-    simp, rintros rfl rfl ⟨⟨q₂, u₂⟩, q'₂, u'₂⟩ mem₂,
-    simp, rintros rfl rfl, simp },
-  refine deterministic.union this (sentence.fix_q.deterministic _ _) _,
-  rintros w₁ w₂ (⟨⟨⟨q, w⟩, ⟨q', w'⟩⟩, mem, rfl⟩ | ⟨⟨⟨q, w⟩, ⟨q', w'⟩⟩, mem, rfl⟩) ⟨_, _⟩,
-  { simp, rintros rfl, exfalso, simpa using proper _ _ mem },
-  { simp }
-end
-
-lemma time_reductions.dsum_aux  {σ : sentence Γ Q ι} {τ : sentence Γ R ι} {n₁ n₂ : ℕ} {m₁ : model Γ Q ι} {L : vector (line Γ) ι} {m₂ : model Γ R ι}
-  (h₁ : m₁ ⟶^(n₁)[σ] ⟨halt, L⟩) (h₂ : ⟨start, L⟩ ⟶^(n₂)[τ] m₂) :
-  m₁.map_q sum.inl ⟶^(n₁ + n₂ + 1)[σ ⨁ τ] m₂.map_q sum.inr :=
-begin
-  have h₁ : m₁.map_q sum.inl ⟶^(n₁)[σ ⨁ τ] ⟨sum.inl halt, L⟩,
-  { have : m₁.map_q sum.inl ⟶^(n₁)[word.map_q (sum.inl : Q → Q ⊕ R) '' σ] ⟨sum.inl halt, L⟩,
-      by simpa using h₁.map_q (sum.inl : Q → Q ⊕ R),
-    refine this.of_ss (by { simp[sentence.dsum, -set.image_subset_iff], 
-      refine set.subset_union_of_subset_left (set.subset_union_left _ _) _ }) },
-  have h : ⟨sum.inl halt, L⟩ ⟶¹[σ ⨁ τ] ⟨sum.inr start, L⟩,
-  { have : ⟨sum.inl halt, L⟩ ⟶¹[sentence.fix_q (sum.inl (halt : Q)) (sum.inr (start : R))] ⟨sum.inr start, L⟩,
-      from sentence.fix_q_reduction (sum.inl halt) (sum.inr start) L,
-    refine this.of_ss (by simp[sentence.dsum, -set.image_subset_iff]) },
-  have h₂ :  ⟨sum.inr start, L⟩ ⟶^(n₂)[σ ⨁ τ] m₂.map_q sum.inr,
-  { have : ⟨sum.inr start, L⟩ ⟶^(n₂)[word.map_q (sum.inr : R → Q ⊕ R) '' τ] m₂.map_q sum.inr,
-      by simpa using h₂.map_q (sum.inr : R → Q ⊕ R),
-    refine this.of_ss (by { simp[sentence.dsum, -set.image_subset_iff], 
-      refine set.subset_union_of_subset_left (set.subset_union_right _ _) _ }) },
-  simpa[show n₁.succ + n₂ = n₁ + n₂ + 1, by omega] using (h₁.succ h).add h₂,
-end
-
-lemma time_reductions.dsum  {σ : sentence Γ Q ι} {τ : sentence Γ R ι} {n₁ n₂ : ℕ} {L₁ L₂ L₃ : vector (line Γ) ι}
-  (h₁ : ⟨start, L₁⟩ ⟶^(n₁)[σ] ⟨halt, L₂⟩) (h₂ : ⟨start, L₂⟩ ⟶^(n₂)[τ] ⟨halt, L₃⟩) :
-  ⟨start, L₁⟩ ⟶^(n₁ + n₂ + 1)[σ ⨁ τ] ⟨halt, L₃⟩ :=
-time_reductions.dsum_aux h₁ h₂
-
-
-lemma reduction_of_fn 
-
-
-end model
-/--/
-variables {Γ Q ι} 
-def deterministic (σ : sentence Γ Q ι) : Prop := ∀ {q q₁ q₂}, q ▷ q₁ ∈ σ → q ▷ q₂ ∈ σ → q₁ = q₂
-
-namespace deterministic
-variables {σ : sentence Γ Q ι} {m₁ m₂ : model Γ Q ι}
-
-lemma reduction (d : deterministic σ) {m m₁ m₂}
-  (h₁ : m ⟶¹[σ] m₁) (h₂ : m ⟶¹[σ] m₂) : m₁ = m₂ :=
-begin
-  rcases h₁ with ⟨_, q₁, z₁, w₁⟩,
-  rcases h₂ with ⟨_, q₂, z₂, w₂⟩,
-  have : q₁ = q₂ ∧ z₁ = z₂, by simpa using d w₁ w₂,
-  rcases this with ⟨rfl, rfl, rfl⟩,
-  refl
-end
-
-lemma time_reductions (d : deterministic σ) {m m₁ m₂} {s} (h₁ : m ⟶^(s)[σ] m₁) (h₂ : m ⟶^(s)[σ] m₂) :
-  m₁ = m₂ :=
-begin
-  induction s with s IH generalizing m₁ m₂,
-  { rcases h₁, rcases h₂, refl },
-  { rcases h₁ with (_ | ⟨_, _, m₁₁, _, h_₁₁, h₁₁_₁⟩),
-    rcases h₂ with (_ | ⟨_, _, m₂₁, _, h_₂₁, h₂₁_₂⟩),
-    have : m₁₁ = m₂₁, from IH h_₁₁ h_₂₁, rcases this with rfl,
-    exact reduction @d h₁₁_₁ h₂₁_₂ }
-end
-
-end deterministic
-
-namespace TM
-variables [state Q] 
-
-instance : inhabited (tape (language Γ)) := ⟨⟨λ n, match n with | 0 := ␤ | (n + 1) := ␣ end, 0⟩⟩
-
-@[simp] lemma tape.default_head : (default : tape (language Γ)).head = 0 := rfl
-
-@[simp] lemma tape.default_tape_0 : (default : tape (language Γ)).tape 0 = ␤ := rfl
-
-@[simp] lemma tape.default_tape_gt0 {n} (h : n > 0) : (default : tape (language Γ)).tape n = ␣ :=
-by { cases n, { simp at h, contradiction }, { refl } }
-
-instance : inhabited (model (language Γ) Q ι) := ⟨⟨vector.repeat default ι, state.start⟩⟩
-
-@[simp] lemma model.default_state : (default : model (language Γ) Q ι).state = state.start := rfl
-
-@[simp] lemma model.default_lines : (default : model (language Γ) Q ι).lines = vector.repeat default ι := rfl
+section TM
 
 def tape_of (x : list Γ) : ℕ → language Γ
 | 0       := ␤
@@ -421,56 +214,234 @@ by { cases n, { simp at h, contradiction },
 structure time_bounded_computable_by_NDTM (f : list Γ → list Γ) (T : ℕ → ℕ) :=
 (Q : Type*)
 (Q_fin : finite Q)
-(Q_state : state Q)
+(Q_state : state_lang Q)
 (σ : sentence (language Γ) Q ι.succ.succ)
 (reduction : ∀ (X : list Γ), 
-  ⟨⟨tape_of X, 0⟩ ::ᵥ vector.repeat default ι.succ, state.start⟩ ⟶^(≤ T X.length)[σ]↓
-  ⟨vector.concat (vector.repeat default ι.succ) ⟨tape_of (f X), 0⟩, state.halt⟩)
-
-structure time_bounded_computable_by_TM (f : list Γ → list Γ) (T : ℕ → ℕ) :=
-(Q : Type*)
-(Q_fin : finite Q)
-(Q_state : state Q)
-(σ : sentence (language Γ) Q ι.succ.succ)
-(deterministic : deterministic σ)
-(reduction : ∀ (X : list Γ), 
-  ⟨⟨tape_of X, 0⟩ ::ᵥ vector.repeat default ι.succ, state.start⟩ ⟶^(≤ T X.length)[σ]↓
-  ⟨vector.concat (vector.repeat default ι.succ) ⟨tape_of (f X), 0⟩, state.halt⟩)
-
-
-
-
-variables {σ : sentence (language Γ) Q ι.succ}
-/--/
-
+  model.is_halt_in_step σ (T X.length) (⟦start, tape_of X ::ᵥ default, default⟧) ∧
+  ⟦start, tape_of X ::ᵥ default, default⟧ ⟶^(≤ T X.length)[σ]↓ ⟦halt, vector.concat default (tape_of (f X)), default⟧)
 
 
 structure time_bounded_computable_by_TM (f : list Γ → list Γ) (T : ℕ → ℕ) :=
 (Q : Type*)
 (Q_fin : finite Q)
-(Q_inhabited : inhabited Q)
-(σ : sentence (language Γ) Q ι.succ)
-(deterministic : deterministic σ)
-(reduction : ∀ (X : list Γ), encode X ⟶^(≤ T X.length)[σ]↓ encode (f X))
-
-def time_bounded_computable_by_TM (f : list Γ → list Γ) (T : ℕ → ℕ) : Prop :=
-  ∃ (c : ℕ) (Q : Type*) [fintype Q] (σ : sentence (language Γ) (state Q) (indexical empty) TM.tape)
-  deterministic σ ∧
-  ∀ (X : list Γ), ∃ (m : model (language Γ) (state Q) (indexical empty) TM.tape),
-  is_terminal (f X) m ∧ (initial X ⟶^(≤ c * T X.length)[σ]↓ m)
-
-lemma constant_computable_by_c : time_bounded_computable_by_TM (λ x : list bool, []) (λ ι, 0) :=
-begin
-  refine ⟨1, empty, fintype_of_option, ∅, by { intros _, simp }, λ X, _⟩,
-  simp, refine ⟨_, 0, by refl, _⟩,
-  { intros _ h,
-    exfalso,
-    rcases h with ⟨_, _, _, _, _, h⟩,
-    exact h },
-  {  }
-end
+(Q_state : state_lang Q)
+(σ : sentence (language Γ) Q ι.succ.succ)
+(deterministic : σ.deterministic)
+(reduction : ∀ (X : list Γ), 
+  ⟦start, tape_of X ::ᵥ default, default⟧ ⟶^(≤ T X.length)[σ]↓ ⟦halt, vector.concat default (tape_of (f X)), default⟧)
 
 end TM
 
+namespace sentence
+open model sentence.deterministic relation
+variables {R : Type*} [state_lang R] (f : Q → R) {σ : sentence Γ Q ι}
+
+@[simp] def word.map_q : word Γ Q ι → word Γ R ι
+| ⟮c, z; u | q, x⟯ := ⟮f c, z; u | f q, x⟯
+
+@[simp] def map_q (σ : sentence Γ Q ι) (f : Q → R) (H : ∀ c z u q x, ⟮c, z; u | q, x⟯ ∈ σ → f q ≠ halt ∧ f c ≠ start) :
+  sentence Γ R ι :=
+{ carrier := word.map_q f '' σ,
+  proper' := by { rintros c z u q x ⟨⟨c', z', u', q', x'⟩, h, eqn⟩,
+                  simp at eqn, rcases eqn with ⟨rfl, rfl, rfl, rfl, rfl⟩, exact H _ _ _ _ _ h } }
+
+end sentence
+
+namespace model
+open sentence sentence.deterministic relation
+variables {m₁ m₂ m₃ : model Γ Q ι} {σ : sentence Γ Q ι}
+
+@[simp] lemma reduct_tape_read {T : vector (ℕ → Γ) ι} {H : vector ℕ ι} : reduct_tape T H (read T H) = T :=
+by { ext, simp, rintros rfl, refl }
+
+@[simp] lemma reduct_head_default {H : vector ℕ ι} : reduct_head H default = H :=
+by { ext, simp, }
+
+lemma reduction.iff {q₁ q₂ : Q} {T₁ T₂ : vector (ℕ → Γ) ι} {H₁ H₂ : vector ℕ ι}  :
+  (⟦q₁, T₁, H₁⟧ ⟶¹[σ] ⟦q₂, T₂, H₂⟧) ↔
+  (∃ (z : vector Γ ι) (u : vector instruction ι), ⟮q₂, z; u | q₁, read T₁ H₁⟯ ∈ σ ∧ T₂ = reduct_tape T₁ H₁ z ∧ H₂ = reduct_head H₁ u) :=
+⟨by { rintros ⟨_, _, _, _, z, u, mem⟩, refine ⟨z, u, mem, rfl, rfl⟩ },
+ by { rintros ⟨z, u, mem, rfl, rfl⟩, refine ⟨_, _, _, _, z, u, mem⟩ }⟩
+
+@[simp] lemma time_bounded_reductions.refl {s} : m₁ ⟶^(≤ s)[σ] m₁ := power_le.refl
+
+@[simp] lemma time_reductions.refl : m₁ ⟶^(0)[σ] m₁ := power.zero _
+
+lemma time_bounded_reductions.of_le {s₁ s₂} (le : s₁ ≤ s₂) (h : m₁ ⟶^(≤ s₁)[σ] m₂) :
+  m₁ ⟶^(≤ s₂)[σ] m₂ := power_le.of_le le h
+
+lemma time_reductions.add {s₁ s₂} (h₁ : m₁ ⟶^(s₁)[σ] m₂) (h₂ : m₂ ⟶^(s₂)[σ] m₃) :
+  m₁ ⟶^(s₁ + s₂)[σ] m₃ := power.add h₁ h₂
+
+lemma time_bounded_reductions.add {s₁ s₂} (h₁ : m₁ ⟶^(≤ s₁)[σ] m₂) (h₂ : m₂ ⟶^(≤ s₂)[σ] m₃) :
+  m₁ ⟶^(≤ s₁ + s₂)[σ] m₃ := power_le.add h₁ h₂
+
+lemma time_bounded_reductions.sum {m : ℕ → model Γ Q ι} {s : ℕ → ℕ}
+  (h : ∀ k, m k ⟶^(≤ s k)[σ] m (k + 1)) (k : ℕ) : (m 0) ⟶^(≤ ∑ i in finset.range k, s i)[σ] (m k) :=
+by { induction k with k IH, { simp }, { simpa[finset.sum_range_succ] using IH.add (h k) } }
+
+lemma reduction.of_ss (r : m₁ ⟶¹[σ] m₂) {τ : sentence Γ Q ι} (ss : σ ≤ τ) : m₁ ⟶¹[τ] m₂ :=
+by { rcases r with ⟨q, T, H, c, z, u, mem⟩, refine ⟨_, _, _, _, _, _, ss mem⟩ }
+
+lemma time_reductions.of_ss {n} (r : m₁ ⟶^(n)[σ] m₂) {τ : sentence Γ Q ι} (ss : σ ≤ τ) : m₁ ⟶^(n)[τ] m₂ :=
+by { induction n with n IH generalizing m₂, { rcases r, simp },
+     { rcases r with (_ | ⟨_, _, m₁₁, _, r₁_₁₁, r₁₁_₂⟩), exact (IH r₁_₁₁).succ (r₁₁_₂.of_ss ss) } }
+
+lemma time_bounded_reductions.of_ss {k} (r : m₁ ⟶^(≤ k)[σ] m₂) {τ : sentence Γ Q ι} (ss : σ ≤ τ) : m₁ ⟶^(≤ k)[τ] m₂ :=
+by { rcases r with ⟨n, le, r⟩, refine ⟨n, le, time_reductions.of_ss r ss⟩ }
+
+section
+variables {R : Type*} [state_lang R] (f : Q → R)
+
+@[simp] def map_q : model Γ Q ι → model Γ R ι
+| ⟦q, T, H⟧ := ⟦f q, T, H⟧
+
+instance [has_coe Q R] : has_coe (model Γ Q ι) (model Γ R ι) := ⟨λ m, m.map_q coe⟩ 
+
+variables (m m' : model Γ Q ι) {f}
+
+@[simp] lemma map_q_tape (m : model Γ Q ι) : (m.map_q f).tape = m.tape := by cases m; simp
+
+@[simp] lemma map_q_head (m : model Γ Q ι) : (m.map_q f).head = m.head := by cases m; simp
+
+@[simp] lemma map_q_state (m : model Γ Q ι) : (m.map_q f).state = f m.state := by cases m; simp
+
+variables (f)
+
+lemma reduction.map_q {H} (h : m₁ ⟶¹[σ] m₂) : m₁.map_q f ⟶¹[σ.map_q f H] m₂.map_q f :=
+by { rcases h with ⟨q, T, H, c, z, u, mem⟩, simp, refine ⟨_, _, _, _, _, _, _⟩, simp[sentence.mem_def], refine ⟨_, mem, by simp⟩ }
+
+lemma time_reductions.map_q {H} {n} (h : m₁ ⟶^(n)[σ] m₂) : m₁.map_q f ⟶^(n)[σ.map_q f H] m₂.map_q f :=
+by { induction n with n IH generalizing m₂, { rcases h, simp },
+     { rcases h with (_ | ⟨_, _, m₁₁, _, r₁_₁₁, r₁₁_₂⟩), refine (IH r₁_₁₁).succ (r₁₁_₂.map_q f) } }
+
+lemma time_bounded_reduction.map_q {H} {k} (h : m₁ ⟶^(≤ k)[σ] m₂) : m₁.map_q f ⟶^(≤ k)[σ.map_q f H] m₂.map_q f :=
+by { rcases h with ⟨n, le, r⟩, refine ⟨n, le, time_reductions.map_q f r⟩ }
+
+variables {f}
+
+lemma deterministic.map_q {H} (inj : function.injective f) (d : deterministic σ) : deterministic (σ.map_q f H) :=
+begin
+  rintros r x d₁ d₂ z₁ z₂ u₁ u₂ h₁ h₂,
+  rcases h₁ with ⟨⟨c₁, z₁', u₁', q₁, x₁'⟩, mem₁, eq₁⟩,
+  have : f c₁ = d₁ ∧ z₁ = z₁' ∧ u₁ = u₁' ∧ f q₁ = r ∧ x = x₁', { simp at eq₁, simp[eq₁] },
+  rcases this with ⟨rfl, rfl, rfl, rfl, rfl⟩,
+  rcases h₂ with ⟨⟨c₂, z₂', u₂', q₂, x₂'⟩, mem₂, eq₂⟩,
+  have : f c₂ = d₂ ∧ z₂ = z₂' ∧ u₂ = u₂' ∧ f q₁ = f q₂ ∧ x = x₂', { simp at eq₂, simp[eq₂] },
+  rcases this with ⟨rfl, rfl, rfl, eqn, rfl⟩,
+  have : q₁ = q₂, from (inj eqn), rcases this with rfl,
+  simp [d mem₁ mem₂]
+end
+
+end
+
+variables {R : Type v} [state_lang R]
+
+namespace sentence
+variables {Q R} (q c : Q) (h : q ≠ halt ∧ c ≠ start) 
+
+inductive fix_q_aux : word Γ Q ι → Prop
+| intro : ∀ (z : vector Γ ι), fix_q_aux ⟮c, z; default | q, z⟯
+
+def fix_q (q c : Q) (h : q ≠ halt ∧ c ≠ start) : sentence Γ Q ι :=
+{ carrier := fix_q_aux q c,
+  proper' := λ c' z u q' x, by { rintros ⟨⟩, exact h } } 
+
+@[simp] lemma fix_q_mem (z : vector Γ ι) :
+  ⟮c, z; default | q, z⟯ ∈ (fix_q q c h : sentence Γ Q ι) :=
+fix_q_aux.intro _
+
+lemma fix_q.deterministic : deterministic (fix_q q c h : sentence Γ Q ι) :=
+by { rintros q' x c₁ c₂ z₁ z₂ u₁ u₂ h₁ h₂, rcases h₁, rcases h₂, simp }
+
+@[simp] lemma fix_q_reduction (T : vector (ℕ → Γ) ι) (H : vector ℕ ι) : ⟦q, T, H⟧ ⟶¹[fix_q q c h] ⟦c, T, H⟧ :=
+reduction.iff.mpr ⟨read T H, default, by simp, by simp⟩
+
+instance : has_union (sentence Γ Q ι) := ⟨λ σ τ,
+{ carrier := σ ∪ τ,
+  proper' := by { rintros c z u q x (h | h), { exact σ.proper h }, { exact τ.proper h } } }⟩
+
+def deterministic.union {σ τ : sentence Γ Q ι} (d₁ : deterministic σ) (d₂ : deterministic τ) 
+  (h : ∀ {q x c₁ c₂ z₁ z₂ u₁ u₂}, ⟮c₁, z₁; u₁ | q, x⟯ ∈ σ → ⟮c₂, z₂; u₂ | q, x⟯ ∈ τ → c₁ = c₂ ∧ z₁ = z₂ ∧ u₁ = u₂) : deterministic (σ ∪ τ) :=
+begin
+  rintros q x c₁ c₂ z₁ z₂ u₁ u₂ (h₁ | h₁) (h₂ | h₂),
+  { exact d₁ h₁ h₂ }, { exact h h₁ h₂ }, { simp [h h₂ h₁] }, { exact d₂ h₁ h₂ }
+end
+
+def dsum_suml (σ : sentence Γ Q ι) : sentence Γ (Q ⊕ R) ι := σ.map_q sum.inl (by { intros _ _ _ _ _ h, unfold halt start, simp[σ.proper h] })
+
+def dsum_sumr (τ : sentence Γ R ι) : sentence Γ (Q ⊕ R) ι := τ.map_q sum.inr (by { intros _ _ _ _ _ h, unfold halt start, simp[τ.proper h] })
+
+def dsum (σ : sentence Γ Q ι) (τ : sentence Γ R ι) : sentence Γ (Q ⊕ R) ι :=
+(σ.map_q sum.inl (by { intros _ _ _ _ _ h, unfold halt start, simp[σ.proper h] })) ∪
+(τ.map_q sum.inr (by { intros _ _ _ _ _ h, unfold halt start, simp[τ.proper h] })) ∪
+(fix_q (sum.inl (halt : Q)) (sum.inr (start : R)) (by unfold halt start; simp))
+
+infix ` ⨁ `:80 := dsum
+
+lemma dsum.deterministic {σ : sentence Γ Q ι} {τ : sentence Γ R ι}
+  (d₁ : deterministic σ) (d₂ : deterministic τ) : deterministic (σ ⨁ τ) :=
+begin
+  refine (deterministic.union (deterministic.union (deterministic.map_q sum.inl_injective d₁) (deterministic.map_q sum.inr_injective d₂) _)
+           (fix_q.deterministic _ _ _) _),
+  { rintros (q | r) _ _ _ _ _ _ _ ⟨⟨c₁, z₁, u₁, q, x⟩, mem₁, eqn₁⟩ ⟨⟨c₂, z₂, u₂, q', x'⟩, mem₂, eqn₂⟩,
+    { simp at eqn₂, contradiction },
+    { simp at eqn₁, contradiction } },
+  { rintros _ _ _ _ _ _ _ _ (⟨⟨c, z, u, q, x⟩, mem, eqn⟩ | ⟨⟨c, z, u, q, x⟩, mem, eqn⟩) ⟨⟩,
+    { simp at eqn, rcases eqn with ⟨rfl, rfl, rfl, rfl, rfl⟩, exfalso, simpa using mem },
+    { simp at eqn, contradiction } }
+end
+
+end sentence
+
+lemma time_reductions.dsum_aux  {σ : sentence Γ Q ι} {τ : sentence Γ R ι} {n₁ n₂} {q r T₁ T₂ T₃ H₁ H₂ H₃}
+  (h₁ : ⟦q, T₁, H₁⟧ ⟶^(n₁)[σ] ⟦halt, T₂, H₂⟧) (h₂ : ⟦start, T₂, H₂⟧ ⟶^(n₂)[τ] ⟦r, T₃, H₃⟧) :
+  ⟦sum.inl q, T₁, H₁⟧ ⟶^(n₁ + n₂ + 1)[σ ⨁ τ] ⟦sum.inr r, T₃, H₃⟧ :=
+begin
+  have h₁ : ⟦sum.inl q, T₁, H₁⟧ ⟶^(n₁)[σ ⨁ τ] ⟦sum.inl halt, T₂, H₂⟧,
+  from time_reductions.of_ss (time_reductions.map_q sum.inl h₁)
+    (by { simp[(⨁)], refine set.subset_union_of_subset_left (set.subset_union_left _ _) _,
+          { intros _ _ _ _ _ h, unfold halt start, simp[σ.proper h] } }),
+  have h : ⟦sum.inl halt, T₂, H₂⟧ ⟶¹[σ ⨁ τ] ⟦sum.inr start, T₂, H₂⟧,
+  from reduction.of_ss (sentence.fix_q_reduction _ _ _ _ _)
+    (by { simp[(⨁)], refine set.subset_union_right _ _, { unfold halt start; simp } }),
+  have h₂ : ⟦sum.inr start, T₂, H₂⟧ ⟶^(n₂)[σ ⨁ τ] ⟦sum.inr r, T₃, H₃⟧,
+  from time_reductions.of_ss (time_reductions.map_q sum.inr h₂)
+    (by { simp[(⨁)], refine set.subset_union_of_subset_left (set.subset_union_right _ _) _,
+          { intros _ _ _ _ _ h, unfold halt start, simp[τ.proper h] } }),
+  simpa[show n₁.succ + n₂ = n₁ + n₂ + 1, by omega] using (h₁.succ h).add h₂
+end
+
+lemma time_reductions.dsum  {σ : sentence Γ Q ι} {τ : sentence Γ R ι} {n₁ n₂ : ℕ} {T₁ T₂ T₃ H₁ H₂ H₃}
+  (h₁ : ⟦start, T₁, H₁⟧ ⟶^(n₁)[σ] ⟦halt, T₂, H₂⟧) (h₂ : ⟦start, T₂, H₂⟧ ⟶^(n₂)[τ] ⟦halt, T₃, H₃⟧) :
+  ⟦start,  T₁, H₁⟧ ⟶^(n₁ + n₂ + 1)[σ ⨁ τ] ⟦halt, T₃, H₃⟧ :=
+time_reductions.dsum_aux h₁ h₂
+
+lemma time_bounded_reductions.dsum  {σ : sentence Γ Q ι} {τ : sentence Γ R ι} {k₁ k₂ : ℕ} {T₁ T₂ T₃ H₁ H₂ H₃}
+  (h₁ : ⟦start, T₁, H₁⟧ ⟶^(≤ k₁)[σ] ⟦halt, T₂, H₂⟧) (h₂ : ⟦start, T₂, H₂⟧ ⟶^(≤ k₂)[τ] ⟦halt, T₃, H₃⟧) :
+  ⟦start,  T₁, H₁⟧ ⟶^(≤ k₁ + k₂ + 1)[σ ⨁ τ] ⟦halt, T₃, H₃⟧ :=
+by { rcases h₁ with ⟨n₁, le₁, h₁⟩, rcases h₂ with ⟨n₂, le₂, h₂⟩, refine ⟨n₁ + n₂ + 1, by linarith, time_reductions.dsum h₁ h₂⟩ }
+
+
+end model
+/--/
+namespace sentence
+
+namespace delete
+
+inductive srh
+| start
+| run
+| halt
+
+instance : state_lang srh := ⟨srh.start, srh.halt⟩
+
+inductive main (i : fin ι) : sentence (language Γ) srh ι
+| start : ∀ v, main (⟨start, v⟩ ▷ ⟨srh.run, ⟩)
+| halt : main (⟨srh.run, vector.repeat ␤ ι⟩ ▷ ⟨halt, vector.repeat (␤, instruction.stay) ι⟩)
+
+end delete
+
+end sentence
+
 end turing_machine
-8
