src/vorspiel.lean
@@ -1,17 +1,105 @@
-import tactic data.vector data.vector.zip 
+import tactic data.vector data.vector3 data.vector.zip 
 
 universes u v
 
-def vorspiel : ℕ := 9
-
 namespace vector
-variables {α : Type u} {n : ℕ}
+section
+variables {α : Type*} {n : ℕ}
 
 def concat : vector α n → α → vector α n.succ
 | ⟨l, h⟩ a := ⟨l.concat a, by simp[h]⟩
 
+end
 
+section zip_with3
+
+variables {α β γ δ : Type*} {n : ℕ} (f : α → β → γ → δ)
+
+def zip_with3 (v₁ : vector α n) (v₂ : vector β n) (v₃ : vector γ n) : vector δ n :=
+@vector.zip_with (α × β) γ δ n (λ p z, f p.1 p.2 z) (vector.zip_with (λ x y, (x, y)) v₁ v₂) v₃
+
+@[simp] lemma zip_with3_nth (v₁ : vector α n) (v₂ : vector β n) (v₃ : vector γ n) (i) :
+  (vector.zip_with3 f v₁ v₂ v₃).nth i = f (v₁.nth i) (v₂.nth i) (v₃.nth i) :=
+by simp [vector.zip_with3]
+
+end zip_with3
 
 end vector
 
-#check vector.concat
+namespace relation
+variables {α : Type u} (r : α → α → Prop) {x y z : α}
+
+def deterministic : Prop := ∀ x y z, r x y → r x z → y = z
+
+inductive transitive_closure : α → α → Prop
+| refl : ∀ x, transitive_closure x x
+| trans' : ∀ {x y z}, transitive_closure x y → r y z → transitive_closure x z
+
+attribute [simp, refl] transitive_closure.refl
+
+namespace transitive_closure
+variables {r}
+
+@[trans] lemma trans (hxy : transitive_closure r x y) (hyz : transitive_closure r y z) : transitive_closure r x z :=
+begin
+  induction hyz,
+  case refl { exact hxy },
+  case trans' : _ _ _ _ ry'z' IH { exact (IH hxy).trans' ry'z' }
+end
+
+lemma of_r (h : r x y) : transitive_closure r x y := (transitive_closure.refl x).trans' h
+
+end transitive_closure
+
+inductive power : ℕ → α → α → Prop
+| zero : ∀ x, power 0 x x
+| succ : ∀ {n x y z}, power n x y → r y z → power n.succ x z
+
+attribute [simp, refl] power.zero
+
+namespace power
+variables {r}
+
+lemma add {n m} (hn : power r n x y) (hm : power r m y z) : power r (n + m) x z :=
+by { induction m with m IH generalizing z, { rcases hm, simpa using hn },
+     { rcases hm with (_ | ⟨_, _, v, _, hyv, rvz⟩), simpa using (IH hyv).succ rvz } }
+
+lemma to_trcl {n} (h : power r n x y) : transitive_closure r x y :=
+by { induction n with n IH generalizing y, { rcases h, refl }, { rcases h with (_ | ⟨_, _, v, _, hxv, rvy⟩), exact (IH hxv).trans' rvy } }
+
+@[simp] lemma zero_iff : power r 0 x y ↔ x = y :=
+⟨by { rintros ⟨⟩, refl }, by { rintros rfl, simp }⟩
+
+lemma deterministic {n} (d : deterministic r) : deterministic (power r n) :=
+by { induction n with n IH, { rintros x y z ⟨⟩ ⟨⟩, refl },
+     { rintros x y z (_ | ⟨_, _, v, _, hxv, rvy⟩) (_ | ⟨_, _, w, _, hxw, rwz⟩),
+     have : v = w, from IH x v w hxv hxw, rcases this with rfl,
+     refine d v y z rvy rwz } }
+
+end power
+
+lemma trans_iff_epower : transitive_closure r x y ↔ ∃ n, power r n x y :=
+⟨λ h, by { induction h with _ x y z hxy ryz IH, { refine ⟨0, by refl⟩ }, 
+           { rcases IH with ⟨n, IH⟩, refine ⟨n.succ, IH.succ ryz⟩ } },
+ by { rintros ⟨n, h⟩, refine h.to_trcl }⟩
+
+def power_le (k : ℕ) (x y : α) : Prop := ∃ n ≤ k, power r n x y
+
+namespace power_le
+variables {r}
+
+@[refl, simp] lemma refl {k : ℕ} : power_le r k x x := ⟨0, by simp⟩
+
+lemma of_le {k l : ℕ} (le : k ≤ l) : power_le r k x y → power_le r l x y :=
+by { rintros ⟨n, len, h⟩, refine ⟨n, le_trans len le, h⟩ }
+
+lemma succ {k : ℕ} : power_le r k x y → r y z → power_le r k.succ x z :=
+by { rintros ⟨n, len, hn⟩ ryz, refine ⟨n.succ, nat.succ_le_succ len, hn.succ ryz⟩ }
+
+@[trans] lemma add {k l : ℕ} : power_le r k x y → power_le r l y z → power_le r (k + l) x z :=
+by { rintros ⟨n, len, hn⟩ ⟨m, lem, hm⟩, refine ⟨ n + m, add_le_add len lem, hn.add hm⟩ }
+
+end power_le
+
+end relation
+
